Utils.v
@@ -1,4 +1,8 @@
+Require Import List.
 Require Import Compare_dec.
+
+Require Import Le Lt.
+Require Import Plus Minus.
 
 Definition ap A B (f:A->B) (a1 a2:A) (p:a1 = a2) := match p in _ = a2 return f a1 = f a2 with eq_refl => eq_refl _ end.
 Implicit Arguments ap [A B a1 a2].
@@ -6,8 +10,8 @@ Implicit Arguments ap [A B a1 a2].
 Definition tr A (B:A->Type) (a1 a2:A) (p:a1 = a2) := match p in _ = a2 return B a1->B a2 with eq_refl => fun b=>b end.
 Implicit Arguments tr [A a1 a2].
 
-Definition trid (T1 T2:Type) (p:T1 = T2) := match p in _ = T2 return T1->T2 with eq_refl => fun x=>x end.
-Implicit Arguments trid [T1 T2].
+Definition cast (T1 T2:Type) (p:T1 = T2) := match p in _ = T2 return T1->T2 with eq_refl => fun x=>x end.
+Implicit Arguments cast [T1 T2].
 
 Definition Sinj n m : forall e:S n = S m,n = m := @ap _ _ pred _ _.
 Implicit Arguments Sinj [n m].
@@ -61,3 +65,139 @@ Fixpoint eqd_eq a b : eqd a b->(a = b) := match a,b with
 	S a,S b => fun p:eqd a b=>ap S (eqd_eq a b p)
 end.
 Implicit Arguments eqd_eq [a b].
+
+(* Like rev_append, but moves at most s elements *)
+Fixpoint unzip T s (l l':list T) := match s with
+	O => l' |
+	S s => match l with
+		nil => l' |
+		a :: l => unzip T s l (a :: l')
+	end
+end.
+Implicit Arguments unzip [T].
+
+Lemma minus_n_Sm n : forall m,pred (n - m) = n - S m.
+	induction n;intro.
+
+	reflexivity.
+
+	destruct m.
+		apply minus_n_O.
+
+		apply IHn.
+Qed.
+
+Lemma le_plus_minus_assoc a b c : (c <= b)->(a + (b - c) = a + b - c).
+	intro.
+	apply plus_reg_l with c.
+	rewrite <- le_plus_minus;[| apply le_trans with (1 := H);apply le_plus_r].
+	rewrite plus_assoc.
+	rewrite <- (plus_comm a).
+	rewrite <- plus_assoc.
+	rewrite <- le_plus_minus with (1 := H).
+	reflexivity.
+Qed.
+
+Lemma length_tl T (l:list T) : length (tl l) = pred (length l).
+	destruct l;reflexivity.
+Qed.
+
+Lemma map_ext_In A B (f g:A->B) l : (forall a,In a l->(f a = g a))->(map f l = map g l).
+	induction l;intro.
+
+	reflexivity.
+
+	simpl in H |- *.
+	rewrite <- (H _ (or_introl _ (eq_refl _))).
+	rewrite <- IHl.
+		reflexivity.
+	intros.
+	exact (H _ (or_intror _ H0)).
+Qed.
+
+Lemma skipnSkipAll T (l:list T) : skipn (length l) l = nil.
+	induction l.
+
+	reflexivity.
+
+	exact IHl.
+Qed.
+
+Lemma skipn_consNth T n (d:T) : forall l,(n < length l)->(nth n l d :: skipn (S n) l = skipn n l).
+	induction n;intro;(destruct l;intro;[destruct lt_n_O with (1 := H) |]).
+
+	reflexivity.
+
+	apply IHn.
+	apply lt_S_n with (1 := H).
+Qed.
+
+Lemma seq_In n l : forall s,In n (seq s l)->(s <= n < s + l).
+	induction l;intros;simpl in H.
+
+	destruct H.
+
+	rewrite <- plus_n_Sm.
+	destruct H.
+		rewrite <- H.
+		apply conj with (1 := le_n _).
+		apply (le_plus_l (S s)).
+
+		destruct (IHl _ H).
+		apply conj with (1 := lt_le_weak _ _ H0).
+		exact H1.
+Qed.
+
+Lemma unzip_length T n : forall l l':list T,(n <= length l)->(length (unzip n l l') = n + length l').
+	induction n;intros ? ?.
+
+	intro.
+	reflexivity.
+
+	destruct l;intro.
+		destruct le_Sn_O with (1 := H).
+	simpl in H |- *.
+	rewrite plus_n_Sm.
+	apply IHn.
+	apply le_S_n with (1 := H).
+Qed.
+
+Lemma unzip_consNth T n (d:T) : forall l l',(n < length l)->(nth n l d :: unzip n l l' = unzip (S n) l l').
+	induction n;intros ? ?;(destruct l;intro;[destruct lt_n_O with (1 := H) |]).
+
+	reflexivity.
+
+	apply IHn.
+	apply lt_S_n with (1 := H).
+Qed.
+
+Lemma unzip_nthHi T n l l' (d:T) : forall m,(n <= m)->(n <= length l)->(nth m (unzip n l l') d = nth (m - n) l' d).
+	induction n;intro.
+
+	intros.
+	rewrite <- minus_n_O.
+	reflexivity.
+
+	destruct m;intro.
+		destruct le_Sn_O with (1 := H).
+	intro.
+	rewrite <- unzip_consNth with (d := d) (1 := H0).
+	simpl.
+	apply IHn with (1 := le_S_n _ _ H) (2 := lt_le_weak _ _ H0).
+Qed.
+
+Lemma unzip_nthLo T n m (d:T) : (m < n)->forall l l',(n <= length l)->(nth m (unzip n l l') d = nth (n - S m) l d).
+	intro.
+	induction H as [| n];intros ? ?;(destruct l;intro Hl;simpl in Hl;[destruct le_Sn_O with (1 := Hl) |]).
+
+	simpl unzip.
+	simpl minus.
+	rewrite <- minus_n_n.
+	change (nth O (t :: l) d) with (nth O (t :: l') d).
+	rewrite (minus_n_n m).
+	apply unzip_nthHi with (1 := le_n _) (2 := le_S_n _ _ Hl).
+
+	rewrite <- minus_Sn_m with (1 := H).
+	simpl.
+	apply IHle with (1 := le_S_n _ _ Hl).
+Qed.
